move nat_from_intseq_le_slice_lemma to Lib.ByteSequence

code/experimental/curve25519/Hacl.Impl.Curve25519.Lemmas.fst
@@ -7,6 +7,8 @@ open Lib.ByteSequence
 
 friend Lib.ByteSequence
 
+#set-options "--z3rlimit 50 --max_fuel 1"
+
 let lemma_nat_from_uints64_le_4 b =
   let res = nat_from_intseq_le b in
   assert (res == v b.[0] + pow2 64 * (nat_from_intseq_le_ (Seq.slice b 1 4)));
@@ -15,43 +17,47 @@ let lemma_nat_from_uints64_le_4 b =
   assert (nat_from_intseq_le_ (Seq.slice b 3 4) == v b.[3]);
   assert (res == v b.[0] + pow2 64 * (v b.[1] + pow2 64 * (v b.[2] + pow2 64 * v b.[3])))
 
-val lemma_nat_from_bytes_le_unroll8:
-  #len:size_nat{0 < len /\ 8 * len <= max_size_t} -> b:lseq uint8 (8 * len) -> Lemma
-  (ensures nat_from_intseq_le_ b == nat_from_intseq_le (Seq.slice b 0 8) + pow2 64 * nat_from_intseq_le_ (Seq.slice b 8 (8 * len)))
-let lemma_nat_from_bytes_le_unroll8 #len b = admit()
-  // assert (nat_from_intseq_le_ b == v b.[0] + pow2 8 * nat_from_intseq_le_ (Seq.slice b 1 (8 * len)));
-  // assert (nat_from_intseq_le_ (Seq.slice b 1 (8 * len)) == v b.[1] + pow2 8 * nat_from_intseq_le_ (Seq.slice b 2 (8 * len)));
-  // assert (nat_from_intseq_le_ (Seq.slice b 2 (8 * len)) == v b.[2] + pow2 8 * nat_from_intseq_le_ (Seq.slice b 3 (8 * len)));
-  // assert (nat_from_intseq_le_ (Seq.slice b 3 (8 * len)) == v b.[3] + pow2 8 * nat_from_intseq_le_ (Seq.slice b 4 (8 * len)));
-  // assert (nat_from_intseq_le_ (Seq.slice b 4 (8 * len)) == v b.[4] + pow2 8 * nat_from_intseq_le_ (Seq.slice b 5 (8 * len)));
-  // assert (nat_from_intseq_le_ (Seq.slice b 5 (8 * len)) == v b.[5] + pow2 8 * nat_from_intseq_le_ (Seq.slice b 6 (8 * len)));
-  // assert (nat_from_intseq_le_ (Seq.slice b 6 (8 * len)) == v b.[6] + pow2 8 * nat_from_intseq_le_ (Seq.slice b 7 (8 * len)));
-  // assert (nat_from_intseq_le_ (Seq.slice b 7 (8 * len)) == v b.[7] + pow2 8 * nat_from_intseq_le_ (Seq.slice b 8 (8 * len)));
+val lemma_uints_from_bytes_le0: len:size_nat{8 * len <= max_size_t} -> b:lseq uint8 (8 * len) -> Lemma
+  (forall (i:nat). i < len - 1 ==> (uints_from_bytes_le #U64 #_ #len b).[i + 1] == uint_from_bytes_le (sub b (8 * (i + 1)) 8))
+let lemma_uints_from_bytes_le0 len b = ()
 
-val lemma_uints64_from_bytes_le_slice:
-  #len:size_nat{8 * len <= max_size_t} -> b:lseq uint8 (8 * len) -> i:size_nat{i <= len} -> Lemma
-  (ensures (
-    Seq.slice (uints_from_bytes_le #U64 #_ #len b) i len ==
-    uints_from_bytes_le #U64 #_ #(len - i) (Seq.slice b (8 * i) (8 * len))))
-let lemma_uints64_from_bytes_le_slice #len b i = admit()
+val lemma_uints_from_bytes_le1: len:size_nat{0 < len /\ 8 * len <= max_size_t} -> b:lseq uint8 (8 * len) -> Lemma
+  (forall (i:nat). i < len - 1 ==> Seq.index (Seq.slice (uints_from_bytes_le #U64 #_ #len b) 1 len) i == uint_from_bytes_le (sub b (8 * (i + 1)) 8))
+let lemma_uints_from_bytes_le1 len b =
+  lemma_uints_from_bytes_le0 len b
 
-#set-options "--z3rlimit 50"
+val lemma_uints_from_bytes_le_slice: len:size_nat{0 < len /\ 8 * len <= max_size_t} -> b:lseq uint8 (8 * len) -> Lemma
+  (Seq.slice (uints_from_bytes_le #U64 #_ #len b) 1 len == uints_from_bytes_le #U64 #_ #(len-1) (Seq.slice b 8 (8 * len)))
+let lemma_uints_from_bytes_le_slice len b =
+  let r = uints_from_bytes_le #U64 #_ #len b in
+  let r1 = uints_from_bytes_le #U64 #_ #(len-1) (Seq.slice b 8 (8 * len)) in
+  assert (forall (i:nat). i < len - 1 ==> r1.[i] == uint_from_bytes_le (sub b (8 * (i + 1)) 8));
+  lemma_uints_from_bytes_le1 len b;
+  eq_intro (Seq.slice r 1 len) r1
+
+val lemma_uints64_from_bytes_le_nat0: len:size_nat{0 < len /\ 8 * len <= max_size_t} -> b:lseq uint8 (8 * len) -> Lemma
+  (nat_from_intseq_le_ (uints_from_bytes_le #U64 #_ #len b) ==
+   nat_from_intseq_le_ (Seq.slice b 0 8) + pow2 64 * nat_from_intseq_le_ (uints_from_bytes_le #U64 #_ #(len-1) (Seq.slice b 8 (8 * len))))
+let lemma_uints64_from_bytes_le_nat0 len b =
+  let r = uints_from_bytes_le #U64 #_ #len b in
+  let r2 : lseq uint64 (len - 1) = Seq.slice r 1 len in
+  let b1 : lseq uint8 (8 * (len - 1)) = Seq.slice b 8 (8 * len) in
+  let r1 = uints_from_bytes_le #U64 #_ #(len-1) b1 in
+  lemma_uints_from_bytes_le_slice len b;
+  assert (nat_from_intseq_le_ r == v r.[0] + pow2 64 * nat_from_intseq_le_ r2);
+  assert (nat_from_intseq_le_ (Seq.slice b 0 8) == v r.[0])
 
 val lemma_uints64_from_bytes_le_nat_:
   #len:size_nat{8 * len <= max_size_t} -> b:lseq uint8 (8 * len) -> Lemma
-  (ensures  nat_from_intseq_le_ (uints_from_bytes_le #U64 #_ #len b) == nat_from_intseq_le_ b)
+  (ensures nat_from_intseq_le_ (uints_from_bytes_le #U64 #_ #len b) == nat_from_intseq_le_ b)
 let rec lemma_uints64_from_bytes_le_nat_ #len b =
   if len = 0 then ()
   else begin
     let b1 = Seq.slice b 8 (8 * len) in
     lemma_uints64_from_bytes_le_nat_ #(len - 1) b1;
     assert (nat_from_intseq_le_ (uints_from_bytes_le #U64 #_ #(len-1) b1) == nat_from_intseq_le_ b1);
-    lemma_nat_from_bytes_le_unroll8 #len b;
-    assert (nat_from_intseq_le_ b == nat_from_intseq_le (Seq.slice b 0 8) + pow2 64 * (nat_from_intseq_le_ (uints_from_bytes_le #U64 #_ #(len-1) b1)));
-    let b64 = uints_from_bytes_le #U64 #_ #len b in
-    assert (v b64.[0] == nat_from_intseq_le (Seq.slice b 0 8));
-    lemma_uints64_from_bytes_le_slice #len b 1;
-    assert (Seq.slice b64 1 len == uints_from_bytes_le #U64 #_ #(len - 1) b1)
+    nat_from_bytes_le_slice_lemma #_ #(8 * len) b 8;
+    lemma_uints64_from_bytes_le_nat0 len b
   end
 
 let lemma_uints64_from_bytes_le_nat #len b = lemma_uints64_from_bytes_le_nat_ #len b
